#+TITLE: Chapter 3.2

* ch3.2
** 3.2-1
   - If \(m \leq n\), then
     \begin{align*}
     f(m)+g(m)&\leq f(n)+g(m)\\
              &\leq f(n)+g(n)
     \end{align*}
     \begin{align*}
     f(g(m))\leq f(g(n))
     \end{align*}
     So \(f(n) + g(n)\) and \(f(g(n))\) are monotonically increasing functions.
   - If \(m \leq n\), then
     \begin{align*}
     f(m)\cdot g(m)&\leq f(n)\cdot g(m)\\
                   &\leq f(n)\cdot f(n)
     \end{align*}
     So \(f(n)\cdot g(n)\) is monotonically increasing.
** 3.2-2
   \begin{align*}
   a^{\log_b c}&=a^{\frac{\log_a c}{\log_a b}}\\
               &=(a^{\log_a c})^{\frac{1}{\log_a b}}\\
               &=c^{\frac{1}{\log_a b}}\\
               &=c^{\log_b a}
   \end{align*}
** 3.2-3
   - According to Stirlingâ€™s approximation, we have
     \begin{align*}
     \lg(n!)&=\lg(\sqrt{2\pi n})+\lg((\frac{n}{e})^n)
              +\lg(1+\Theta(\frac{1}{n}))\\
            &=\Theta(\lg n)+\Theta(n\lg n)+\Theta(1/n)\\
            &=\Theta(n\lg n)
     \end{align*}
   - For any positive constant c > 0, when \(n \geq n_0 > 4\,c\), we have
     \begin{align*}
     n!&=n\prod_{i=2}^{n-1}i\\
       &>4\,c\prod_{i=2}^{n-1}i\\
       &\geq 4\,c\prod_{i=2}^{n-1}2\\
       &=c\,2^n
     \end{align*}
     So \(n! = \omega(2^n)\).
   - For any positive constant c > 0, when \(n \geq n_0 > \frac{1}{c}\), we have
     \begin{align*}
     n!&=\prod_{i=2}^{n}i\\
       &\leq \prod_{i=2}^{n}n\\
       &=n^{n-1}\\
       &< c\,n^n
     \end{align*}
     So \(n! = o(n^n)\).
** 3.2-4
   - \(\lceil \lg n \rceil !\) is not polynomial bounded.
     \begin{align*}
     \lceil\lg{n}\rceil!
       &\geq(\lg{n})!\\
       &=\sqrt{2\pi\lg{n}}(\frac{\lg{n}}{e})^{\lg{n}}
         (1+\Theta(\frac{1}{\lg{n}}))\\
       &=\Theta((\lg{n})^{\lg{n}+\frac{1}{2}})\\
       &=\omega((2^k)^{\lg{n}})&&\text{k is a positive constant}\\
       &=\omega(n^k)
     \end{align*}
   - \(\lceil \lg\lg n \rceil !\) is polynomial bounded.

     \(\exists c \in \mathbb{R}^{+}\) s.t.
     \(c\lg\lg n \geq \lceil \lg\lg n \rceil\),
     let \(x = c\lg\lg n\),
     \begin{align*}
     \lceil\lg{\lg{n}}\rceil!
       &\leq x!\\
       &=\sqrt{2\pi x}(\frac{x}{e})^x(1+\Theta(\frac{1}{x}))\\
       &=\sqrt{x}\Theta(x^x)\\
       &=2^{\Theta(x\lg{x})}\\
       &=2^{o(2^x)}\\
       &=o(n^k)&&\text{k is a positive constant}
     \end{align*}
** 3.2-5
   \(\lg^*(\lg{n})\) is asymptotically larger.
   \begin{align*}
   \lg^*(\lg{n})
     &=\lg^*{n}-1\\
     &=\omega(\lg(\lg^*n))
   \end{align*}
** 3.2-6
   - \(\phi = \frac{1 + \sqrt{5}}{2}\)
     \begin{align*}
     \phi^2
       &=(\frac{1+\sqrt{5}}{2})^2\\
       &=\frac{6+2\sqrt{5}}{4}\\
       &=\frac{1+\sqrt{5}}{2}+1\\
       &=\phi+1
     \end{align*}
   - \(\hat{\phi} = \frac{1 - \sqrt{5}}{2}\)
     \begin{align*}
     \hat{\phi}^2
       &=(\frac{1-\sqrt{5}}{2})^2\\
       &=\frac{6-2\sqrt{5}}{4}\\
       &=\frac{1-\sqrt{5}}{2}+1\\
       &=\hat{\phi}+1
     \end{align*}
** 3.2-7
   *Base case:* \(F_1 = \frac{\phi - \hat{\phi}}{2} = 1\),
   \(F_2 = \frac{\phi^2 - \hat{\phi}^2}{2} = 1\)

   *Inductive step:*
   \begin{align*}
   F_{i+2}
     &=F_i+F_{i+1}\\
     &=\frac{\phi^i-\hat{\phi}^i}{\sqrt{5}}
       +\frac{\phi^{i+1}-\hat{\phi}^{i+1}}{\sqrt{5}}\\
     &=\frac{\phi^i(\phi+1)-\hat{\phi}^i(\hat{\phi}+1)}{\sqrt{5}}\\
     &=\frac{\phi^i\phi^2-\hat{\phi}^i\hat{\phi}^2}{\sqrt{5}}\\
     &=\frac{\phi^{i+2}-\hat{\phi}^{i+2}}{\sqrt{5}}
   \end{align*}

   *Finally:* By induction, we prove that
   \(F_i = \frac{\phi^i - \hat{\phi}^i}{\sqrt{5}}\).
** 3.2-8
   - If \(f_1(n) = \Theta(g_1(n))\) and \(f_2(n) = \Theta(g_2(n))\),
     then \(f_1(n) / f_2(n) = \Theta(g_1(n) / g_2(n))\).

     *Proof:*

     \(f_1(n) = \Theta(g_1(n))\), then
     \begin{equation*}
     (\exists c_1,c_2,n_1\in\mathbb{R}^{+})
     [(\forall n\geq n_1)
      [0\leq c_1g_1(n)\leq f_1(n)\leq c_2g_1(n)]]
     \end{equation*}
     \(f_2(n) = \Theta(g_2(n))\), then
     \begin{equation*}
     (\exists c_3,c_4,n_2\in\mathbb{R}^{+})
     [(\forall n\geq n_2)
      [0\leq c_3g_2(n)\leq f_2(n)\leq c_4g_2(n)]]
     \end{equation*}
     therefore
     \begin{equation*}
     (\exists c_1,c_2,c_3,c_4,n_1,n_2\in\mathbb{R}^{+})
     [(\forall n\geq max(n_1,n_2))
      [0\leq \frac{c_1}{c_4}\frac{g_1(n)}{g_2(n)}\leq \frac{f_1(n)}{f_2(n)}
       \leq \frac{c_2}{c_3}\frac{g_1(n)}{g_2(n)}]]
     \end{equation*}
     hence \(f_1(n) / f_2(n) = \Theta(g_1(n) / g_2(n))\).
   - Now we prove that \(k\ln k = \Theta(n)\) implies \(k = \Theta(n / \ln n)\).

     \(k\ln k = \Theta(n)\), so there exists positive constants \(c_1\), \(c_2\)
     and \(n_0\) such that \(0 \leq c_1 n \leq k\ln k \leq c_2 n\).

     Take logarithm of all terms in the inequality, we have
     \(\ln(c_1 n) \leq \ln k + \ln\ln k \leq \ln(c_2 n)\).
     Make k and n large enough, then
     \begin{equation*}
     0 \leq \ln n < \ln(c_1 n) \leq \ln k + \ln\ln k \leq 2\ln k
     \end{equation*}
     \begin{equation*}
     0 \leq \ln k < \ln k + \ln\ln k \leq \ln(c_2 n) \leq 2\ln n
     \end{equation*}
     Hence \(\ln k = \Theta(\ln n)\), so
     \begin{align*}
     k&=\frac{k\ln k}{\ln k}\\
      &=\frac{\Theta(n)}{\Theta(\ln n)}\\
      &=\Theta(\frac{n}{\ln n})
     \end{align*}
